\section{Reliability Analysis} % (fold)
\label{sec:reliability_analysis}

For a continuous random variable $T$ that represents time to failure of a system, the probability of a system failure before time $t$ is

\begin{equation}
  P(T \leq t) = F(t) = \int^t_0 f(u) du
\end{equation}

The reliability function is

\begin{equation}
  R(t) = P(T > t) = 1 - F(t)
\end{equation}

Then, the hazard rate is

\begin{equation}
  h(t) = \frac{f(t)}{R(t)}
\end{equation}


%-------------------------------------------------- 
\subsection{Exponential Failure Model} % (fold)
\label{sub:exponential_failure_model}

\begin{equation}
  f(t) = \begin{cases}
    \lambda e^{-\lambda t} \qquad &\text{for } t \geq 0 \\
    0 \qquad &\text{for } t < 0 \\
  \end{cases}
\end{equation}
\begin{multicols}{2}
\begin{equation}
  F(t) = \int^t_0 f(u) du = 1 - e^{-\lambda t}
\end{equation}
\begin{equation}
  R(t) = e^{-\lambda t}
\end{equation}

\begin{equation}
  H(t) = - \log(R(t))  = \lambda t
\end{equation}

\begin{equation}
  h(t) = \frac{dH(t)}{dt} = \lambda
\end{equation}
\end{multicols}
% subsection exponential_failure_model (end)
%-------------------------------------------------- 


%-------------------------------------------------- 
\subsection{Weibull Failure Model} % (fold)
\label{sub:weibull_failure_model}
\begin{equation}
  f(t) = \begin{cases}
    \lambda \beta(\lambda t)^{\beta-1}e^{-(\lambda t)^\beta} \qquad &\text{for } t \geq 0 \\
    0 \qquad &\text{for } t < 0 \\
  \end{cases}
\end{equation}
\begin{multicols}{2}
  \begin{equation}
    F(t) = \int^t_0 \lambda \beta(\lambda U)^{\beta-1}du = 1 - e^{-(\lambda t)^\beta}
  \end{equation}
  \begin{equation}
    R(t) = e^{-(\lambda t)^\beta}
  \end{equation}
  \begin{equation}
    H(t) = (\lambda t)^{\beta}
  \end{equation}
  \begin{equation}
    h(t) = \beta \lambda (\lambda t)^{\beta-1}
  \end{equation}
\end{multicols}
% subsection weibull_failure_model (end)
%-------------------------------------------------- 

\subsection{System of Components} % (fold)
\label{sub:system_of_components}

\textbf{Series}
\begin{equation}
  R(t) = R_1(t)R_2(t)
\end{equation}

\textbf{Parallel}
\begin{equation}
  R(t) = 1 - [1- R_1(t)][1 - R_2(t)]
\end{equation}

% subsection system_of_components (end)

% section reliability_analysis (end)